VeriMon: refactor conversion-avoiding interface

src/algorithm_verified.ml
@@ -1,33 +1,26 @@
 let no_mw = ref false
 
-module IntMap = Map.Make(struct type t = int let compare = Stdlib.compare end)
-
 module Monitor = struct
-  type ctxt = {
-    c_fv_pos: int list;
-    mutable c_tp: int;
-    mutable c_tpts: MFOTL.timestamp IntMap.t;
-    mutable c_ts: MFOTL.timestamp;
-    mutable c_vst: Verified_adapter.state;
+  type t = {
+    fv_pos: int list;
+    mutable cur_tp: int;
+    mutable cur_ts: MFOTL.timestamp;
+    mutable cur_db: Verified_adapter.db;
+    mutable cur_state: Verified_adapter.state;
   }
 
-  let begin_tp c ts =
-    c.c_ts <- ts;
-    c.c_tpts <- IntMap.add c.c_tp ts c.c_tpts
+  let begin_tp ctxt ts = ctxt.cur_ts <- ts
 
-  let observe c e t =
-    c.c_vst <- Verified_adapter.observe e t c.c_vst
+  let tuple ctxt s sl =
+    ctxt.cur_db <- Verified_adapter.insert_into_db s sl ctxt.cur_db
 
-  let end_tp c =
-    let (vs, new_state) = Verified_adapter.conclude c.c_ts c.c_vst in
-    List.iter (fun (qtp, rel) ->
-        let qts = IntMap.find qtp c.c_tpts in
-        if qts < MFOTL.ts_max then
-          Helper.show_results c.c_fv_pos c.c_tp qtp qts rel
-      ) vs;
-    c.c_tpts <- List.fold_left (fun m (qtp,_) -> IntMap.remove qtp m) c.c_tpts vs;
-    c.c_vst <- new_state;
-    c.c_tp <- c.c_tp + 1
+  let end_tp ctxt =
+    let (vs, new_state) = Verified_adapter.step ctxt.cur_ts ctxt.cur_db ctxt.cur_state in
+    List.iter (fun (q, tsq, rel) ->
+      Helper.show_results ctxt.fv_pos ctxt.cur_tp q tsq rel) vs;
+    ctxt.cur_tp <- ctxt.cur_tp + 1;
+    ctxt.cur_db <- Verified_adapter.empty_db;
+    ctxt.cur_state <- new_state
 end
 
 module P = Simple_log_parser.Make (Monitor)
@@ -40,11 +33,11 @@ let monitor dbschema logfile fv f =
   let cf = Verified_adapter.convert_formula dbschema f in
   let cf = if !no_mw then cf else Verified.Monitor.convert_multiway cf in
   let ctxt = Monitor.{
-    c_fv_pos = fv_pos;
-    c_tp = 0;
-    c_tpts = IntMap.empty;
-    c_ts = MFOTL.ts_invalid;
-    c_vst = Verified_adapter.init cf;
+    fv_pos;
+    cur_tp = 0;
+    cur_ts = MFOTL.ts_invalid;
+    cur_db = Verified_adapter.empty_db;
+    cur_state = Verified_adapter.init cf;
   } in
   let lexbuf = Log.log_open logfile in
   ignore (P.parse dbschema lexbuf ctxt)
