src/verified_adapter.mli
@@ -6,7 +6,10 @@ open Helper
 val is_monitorable: Db.schema -> formula -> bool * (formula * string) option
 val convert_formula: Db.schema -> formula -> Verified.Monitor.formula
 
+type db
+val empty_db: db
+val insert_into_db: Table.schema -> string list -> db -> db
+
 type state
 val init: Verified.Monitor.formula -> state
-val observe: string -> cst list -> state -> state
-val conclude: timestamp -> state -> (int * relation) list * state
+val step: MFOTL.timestamp -> db -> state -> (int * MFOTL.timestamp * relation) list * state
