thys/MFODL_Monitor_Devel/Monitor_Code.thy
@@ -4,18 +4,17 @@ theory Monitor_Code
 begin
 (*>*)
 
-export_code convert_multiway vminit_safe minit_safe vmstep mstep mmonitorable_exec
+export_code convert_multiway mmonitorable_exec vminit_safe minit_safe vmstep mstep
    checking OCaml?
-
 
 export_code
   (*basic types*)
   nat_of_integer integer_of_nat int_of_integer integer_of_int enat
-  interval RBT_set rbt_empty rbt_insert rbt_fold
+  interval empty_db insert_into_db RBT_set rbt_fold
   (*term, formula, and regex constructors*)
   EInt Formula.Var Formula.Agg_Cnt Formula.Pred Regex.Skip Regex.Wild
   (*main functions*)
-  convert_multiway mmonitorable_exec minit_incr mobserve mconclude
+  convert_multiway mmonitorable_exec minit_safe mstep
   in OCaml module_name Monitor file_prefix "verified"
 
 (*<*)
